- Antiderivatives find the function from a given derivative.

Example
---
$$\begin{align}
F(x)&=x^3\\
F'(x)&=3x^2 &&\text{(2)}\\
f(x)&=x^3 &&\text{Is the antiderivative of (2)}
\end{align}$$

* Can also use any arbitrary constant on the end, as it will be dropped when taking the derivative anyways.

Example
---
$$\begin{align}
F(x) &= \frac{x^{p+1}}{p+1} &&\text{(1)}\\
\\
F'(x) &= \frac{1}{p+1}\cdot\left(p+1\right)x^p &&\text{(2)} \\
&= x^p &&\text{(3)}\\
\\
&\text{(1) is the antiderivative of (3).}
\end{align}$$

* The most general antiderivative of $f$ is $F(x) + C$ where $C$ is an arbitrary constant.

Example
---

$$\begin{align}
f(1) &= 1\\
f'(x) &= \frac{1}{\sqrt{x}+3}\\
\\
&= x^{-1\over2}+3x^0 \\
\\
f(x) &= \frac{1}{\frac{-1}{2}+1}x^{1\over2}+3x+C &&\text{The antiderivative}\\
&= 2x^{-1\over2}+3x+C\\
\\
\text{As }f(1) = 1, C = -4.
\end{align}$$
